Require all latches to have a next and init lit

Valaig/Aig/Basic.lean
@@ -3,11 +3,11 @@ import Std.Sat.AIG.CachedGates
 import Valaig.Aig.Defs
 import Valaig.Aig.DefsLemmas
 import Valaig.Aig.RefsLemmas
+import Valaig.ForStd
 
 namespace Valaig.Aig.Raw
 
-@[inline]
-def size (aig : Raw) : Nat := aig.aig.decls.size
+attribute [local simp, local grind] Raw.size
 
 @[inline, simp]
 abbrev numInputs (aig : Raw) : Nat := aig.inputs.size
@@ -34,16 +34,9 @@ def numGates (aig : Raw) : Nat := aig.size - aig.numLeaves
 
 end Aig.Raw
 
-@[inline]
-def Var.validIn (var : Var) (aig : Aig.Raw) : Prop :=
-  var.idx < aig.size
-deriving Decidable
-
 @[inline, simp]
-abbrev Lit.validIn (lit : Lit) (aig : Aig.Raw) := lit.var.validIn aig
-
-abbrev Var.In (aig : Aig.Raw) := { var : Var // var.validIn aig }
-abbrev Lit.In (aig : Aig.Raw) := { lit : Lit // lit.validIn aig }
+private abbrev Lit.In.ref {aig : Aig.Raw} (lit : Lit.In aig) : aig.aig.Ref :=
+  lit.val.toRef (by grind only [Var.validIn_def'])
 
 namespace Aig
 
@@ -76,6 +69,7 @@ def empty : Aig :=
     hfalse := by simp [Std.Sat.AIG.empty],
     hinputs := by simp [Std.Sat.AIG.empty],
     hlatches := by simp [Std.Sat.AIG.empty],
+    hnexts := by simp,
   }
 
 @[inline]
@@ -103,11 +97,13 @@ def addInput (aig : Aig) (symbol : String := "") : Aig × Input :=
       · grind only [mkAtom_ref_eq_decls_size, Var.ofRef_idx]
       · grind only [nextInputIdx]
     hlatches := by apply AtomsBij_unchanged_push (by apply mkAtom_eq_decls_push) <;> grind only [hlatches],
+    hnexts := by grind only [validIn_push aig, mkAtom_eq_decls_push, hnexts]
   }
   (aig, input)
 
 @[inline]
-def addLatch (aig : Aig) (next : Lit) (reset : Option Lit := none) (symbol : String := "") : Aig × Latch :=
+def addLatch (aig : Aig) (next : Lit) (reset : Lit) (symbol : String := "")
+    (hnext : next.validIn aig := by grind) (hreset : reset.validIn aig := by grind) : Aig × Latch :=
   -- We don't need to use mkAtomCached as nextLatchIdx_notIn_decls guarantees
   -- it would be a miss
   let res := aig.aig.mkAtom <| .latch aig.nextLatchIdx
@@ -115,6 +111,7 @@ def addLatch (aig : Aig) (next : Lit) (reset : Option Lit := none) (symbol : Str
     var := .ofRef res.ref,
     next,
     reset,
+    hreset := by simp_all [res, Var.validIn, Var.lt_idx, mkAtom_ref_eq_decls_size, Aig.Raw.size]
     symbol
   }
 
@@ -127,30 +124,7 @@ def addLatch (aig : Aig) (next : Lit) (reset : Option Lit := none) (symbol : Str
       apply AtomsBij_push_push (by apply mkAtom_eq_decls_push) (by trivial) (hbijec := aig.hlatches)
       · grind only [mkAtom_ref_eq_decls_size, Var.ofRef_idx]
       · grind only [nextLatchIdx]
-  }
-  (aig, latch)
-
-@[inline]
-def addLatch' (aig : Aig) (reset : Option Lit := none) (symbol : String := "") : Aig × Latch :=
-  -- We don't need to use mkAtomCached as nextLatchIdx_notIn_decls guarantees
-  -- it would be a miss
-  let res := aig.aig.mkAtom <| .latch aig.nextLatchIdx
-  let latch := {
-    var := .ofRef res.ref,
-    next := none,
-    reset,
-    symbol
-  }
-
-  let aig := { aig with
-    aig := res.aig,
-    latches := aig.latches.push latch,
-    hfalse := by apply hfalse_decls_push ?_ (by apply mkAtom_eq_decls_push) <;> grind only [hfalse],
-    hinputs := by apply AtomsBij_unchanged_push (by apply mkAtom_eq_decls_push) <;> grind only [hinputs],
-    hlatches := by
-      apply AtomsBij_push_push (by apply mkAtom_eq_decls_push) (by trivial) (hbijec := aig.hlatches)
-      · grind only [mkAtom_ref_eq_decls_size, Var.ofRef_idx]
-      · grind only [nextLatchIdx]
+    hnexts := by grind only [validIn_push aig, mkAtom_eq_decls_push, Array.getElem_push, hnexts]
   }
   (aig, latch)
 
@@ -177,6 +151,7 @@ def addGate (aig : Aig) (rhs0 rhs1 : Lit)
       · apply Std.Sat.AIG.mkAndCached_le_size
       · grind only [Std.Sat.AIG.mkAndCached_decl_eq]
       · grind only [mkAndCached_matches_gate],
+    hnexts := by grind only [validIn_of_ge_size aig, Std.Sat.AIG.mkAndCached_le_size, hnexts, Aig.Raw.size]
   }
   (aig, Lit.ofRef res.ref)
 
@@ -203,109 +178,31 @@ def addGateUncached (aig : Aig) (rhs0 rhs1 : Lit)
       · apply Std.Sat.AIG.mkGate_le_size
       · grind only [Std.Sat.AIG.mkGate_decl_eq]
       · grind only [mkGate_matches_gate]
+    hnexts := by grind only [validIn_of_ge_size aig, Std.Sat.AIG.mkGate_le_size, hnexts, Aig.Raw.size]
   }
   (aig, Lit.ofRef res.ref)
 
-@[unbox, grind]
-structure finaliseLatches.State (aig : Aig) where
-  latches : Latches := aig.latches
-  idx : Nat := 0
-  hsize : latches.size = aig.latches.size := by grind
-  habove : ∀ {i} (_hge : i ≥ idx) (hlt : i < latches.size), latches[i] = aig.latches[i] := by grind
-  hvar : ∀ {i} (h : i < latches.size), latches[i].var = aig.latches[i].var := by grind
-
 @[inline]
-def finaliseLatches.State.empty (aig : Aig) : State aig :=
-  {}
-
-@[inline]
-def finaliseLatches (aig : Aig) (nextState : (latch : Latch) -> latch ∈ aig.latches -> Lit.In aig) : Aig :=
-  have s := updateLatches
+def setNext (aig : Aig) (i : LatchIdx) (h : i < aig.numLatches)
+    (next : Lit) (hnext : next.validIn aig := by grind) : Aig :=
+  let latches := aig.latches.modifyMem i h ({ ·.val with next })
   { aig with
-    latches := s.latches,
-    hlatches := by
-      constructor
-      all_goals intro _ h; simp only [s.hvar, s.hsize]
-      · apply aig.hlatches.hinjec
-      · apply aig.hlatches.hsurjec
+    latches,
+    hlatches := by constructor <;> grind [hlatches]
+    hnexts := by grind [hnexts, validIn_of_aig_eq aig]
   }
 
-where
-  updateLatches (s : finaliseLatches.State aig := .empty aig) : finaliseLatches.State aig :=
-    if hidx : s.idx ≥ s.latches.size then
-      s
-    else
-      have next := step s (by omega)
-      have : next.val.latches.size - next.val.idx < s.latches.size - s.idx := by
-        grind only [finaliseLatches.State.hsize]
+@[inline]
+def setNexts (aig : Aig) (f : (latch : Latch) -> latch ∈ aig.latches -> Lit.In aig) : Aig :=
+  let modify _ _ latch _ :=
+    let next := f latch (by grind only [Array.getElem_mem])
+    { latch with next }
 
-      updateLatches next
-  termination_by s.latches.size - s.idx
-
-  step (s : finaliseLatches.State aig) (h : s.idx < s.latches.size) : { s' : finaliseLatches.State aig // s'.idx = s.idx + 1 } :=
-    match s.latches[s.idx].next with
-    -- If the next value is already set, do nothing and continue
-    | some _ =>
-      ⟨{ s with
-        idx := s.idx + 1,
-        habove := by intro i h; exact s.habove (by omega)
-      }, by simp only⟩
-    | none =>
-      -- Otherwise get the current latch, compute its new next state and then
-      -- modify in place
-      let latch := s.latches[s.idx]
-      have hmem : latch ∈ aig.latches := by
-        subst latch; rw [s.habove]; apply Array.getElem_mem; omega
-      let next := nextState latch hmem
-      let latches := s.latches.modify s.idx fun latch => { latch with next }
-
-      ⟨{ s with
-        latches,
-        idx := s.idx + 1,
-
-        hsize := by subst latches; rw [Array.size_modify, s.hsize]
-        habove := by intros; rw [Array.getElem_modify_of_ne]; apply s.habove; all_goals omega
-        hvar := by intros; rw [Array.getElem_modify]; split <;> apply s.hvar
-      }, by simp only⟩
-
-
--- [>-
--- A timeframe in the execution of the model, starting from the initial state at 0
--- -/
--- abbrev Frame := Nat
-
--- structure Entrypoint (α : Type) [DecidableEq α] [Hashable α] where
---   [>-
---   The Aig that we are in.
---   -/
---   aig : Aig α
---   [>-
---   The reference to the node in `aig` that this `Entrypoint` targets.
---   -/
---   ref : aig.Ref
---   [>-
---   The timeframe that this `Entrypoint` targets.
---   -/
---   frame : Frame
-
--- @[inline]
--- def Entrypoint.toAIGEntrypoint (entry : Entrypoint α) : AIG.Entrypoint (Atom α) :=
---   { aig := entry.aig.aig, ref := entry.ref }
-
--- def denote (assign : α -> Frame -> Bool) (entry : Entrypoint α) : Bool :=
---   sorry
--- -- TODO: Reasoning about termination of this is somewhat annoying because of how
--- -- it sends a callback into AIG.denote, is there a better way of formalising this?
--- --     AIG.denote assignAtFrame entry.toAIGEntrypoint
---   -- where
--- --     assignAtFrame (atom : Atom α) : Bool :=
--- --       match atom with
--- --       | .input a => assign a entry.frame
--- --       | .latch idx =>
--- --         let latch := entry.aiger.latches[idx]'(sorry)
--- --         match entry.frame with
--- --         | 0 => denote assign { entry with ref := latch.reset, frame := 0 }
--- --         | Nat.succ n =>  denote assign { entry with ref := latch.next, frame := n - 1 }
+  { aig with
+    latches := aig.latches.mapMem modify
+    hlatches := by constructor <;> grind only [hlatches, Array.size_mapMem, Array.getElem_mapMem]
+    hnexts := by grind only [validIn_of_aig_eq aig, Array.getElem_mapMem]
+  }
 
 end Aig
 
