Valaig/Aig/FromStd.lean
@@ -1,29 +1,36 @@
 import Valaig.Aig.Basic
 import Valaig.Aig.Lemmas
 import Std.Sat.AIG.Basic
+import Valaig.Prelude
 
 -- Convert from a Std.Sat.AIG to our sequential Aig
 
 namespace Valaig.Aig
 
+open Std.Sat AIG
 variable {α : Type} [DecidableEq α] [Hashable α]
 
-open Std.Sat AIG
+namespace FromStd
 
 inductive RelabelledAtom (aig : AIG α) where
-| input (symbol : String := "")
+| input
+  (symbol : String := "")
 | latch
   (next : aig.Ref)
-  (reset : Bool⊕ Option aig.Ref := .inr none)
+  -- TODO: Support generic reset functions and uninitialised latches not just Bool
+  (reset : Bool)
   (symbol : String := "")
 
 @[unbox, grind]
-private structure FromStdState (stdAig : AIG α) where
+private structure State (stdAig : AIG α) where
   aig : Aig := .empty
-  -- A map from variable indices in stdAig (Ref.gate) to Vars in aig
-  map : Array Var := #[]
+
+  -- A map from variable indices in stdAig (Ref.gate) to Lits in aig
+  map : Array Lit := #[]
+
   -- A map from atoms in the original AIG to their canonical variable in aig
   atomMap : Std.HashMap α Var := .emptyWithCapacity
+
   -- A map from the variable defined by each latch to its ref in stdAig, to
   -- allow latch finalisation once all nodes have been visited
   latchNexts : Std.HashMap Var stdAig.Ref := .emptyWithCapacity
@@ -33,114 +40,147 @@ private structure FromStdState (stdAig : AIG α) where
   hatom : ∀ {a} (_ : a ∈ atomMap),
     ∃ (h : atomMap[a].validIn aig), aig[atomMap[a]] matches .atom _ := by grind
 
-structure FromStdResult (stdAig : AIG α) where
+namespace State
+
+variable {aig : AIG α}
+
+@[simp, grind]
+abbrev size (s : State aig) := s.map.size
+
+@[simp, grind]
+def measure (s : State aig) := aig.decls.size - s.size
+
+abbrev Pushed (s : State aig) := { s' : State aig // s'.size = s.size + 1 }
+
+@[always_inline]
+def addFalse (s : State aig) : s.Pushed :=
+  ⟨{ s with map := s.map.push .false, hmap := by grind}, by grind only [Array.size_push]⟩
+
+@[always_inline]
+def addGate (s : State aig) (rhs0 rhs1 : Fanin)
+    (h0 : rhs0.gate < s.map.size) (h1 : rhs1.gate < s.map.size) : s.Pushed :=
+  let rhs0 := s.map[rhs0.gate]'h0 |>.invert rhs0.invert
+  let rhs1 := s.map[rhs1.gate]'h1 |>.invert rhs1.invert
+  rlet (aig, lhs) := s.aig.addGate rhs0 rhs1
+  let map := s.map.push lhs
+
+  have hmap := by grind only [addGate_validIn, validIn_addGate, Array.mem_push]
+  have hlatch := by grind only [addGate_latches_eq]
+  have hatom := by grind only [validIn_addGate, addGate_getElem_eq]
+  ⟨{ s with aig, map, hmap, hlatch, hatom }, by grind only [Array.size_push]⟩
+
+-- Tries to add an atom that already exists, returns none if it doesn't
+@[always_inline]
+def tryAddCachedAtom (s : State aig) (atom : α) : Option s.Pushed := do
+  rlet h : var ← s.atomMap[atom]?
+  let map := s.map.push var.toLit
+
+  have hmap := by
+    simp_all
+    rintro _ (hold | hnew)
+    · exact s.hmap hold
+    · have := Std.HashMap.isSome_getElem?_iff_mem.mp (Option.isSome_of_eq_some h)
+      simp_all; rw [←h]; cases (s.hatom this); trivial
+  return ⟨{ s with map, hmap }, by grind only [Array.size_push]⟩
+
+@[always_inline]
+def addInput (s : State aig) (atom : α) (symbol : String) : s.Pushed :=
+  let (eq:=_) (aig, input) := s.aig.addInput symbol
+  let map := s.map.push input
+  let atomMap := s.atomMap.insert atom input
+
+  have hmap := by simp; grind only [addInput_matches_atom, Lit.mk_self_eq_self, validIn_addInput, Lit.mk_ext]
+  have hlatch := by grind only [addInput_latches_eq]
+  have hatom := by
+    intros
+    simp only [Std.HashMap.getElem_insert]
+    split
+    · grind only [addInput_matches_atom]
+    · grind only [validIn_addInput, addInput_getElem_eq]
+  ⟨{ s with aig, map, atomMap, hmap, hlatch, hatom }, by grind only [Array.size_push]⟩
+
+@[always_inline]
+def addLatch (s : State aig) (atom : α) (next : aig.Ref) (reset : Bool) (symbol : String) : s.Pushed :=
+  let nextLit := Lit.ofRef next
+  let resetLit := Lit.constant reset
+
+  -- We set a fake next state literal at first because we may not have added the logic driving
+  -- the next state yet and store it in latchNexts so we can update it subsequently
+  let (eq:=_) (aig, latch) := s.aig.addLatch .false resetLit symbol
+  let map := s.map.push latch
+  let atomMap := s.atomMap.insert atom latch
+  let latchNexts := s.latchNexts.insert latch next
+
+  have hmap := by simp; grind only [addLatch_matches_atom, Lit.mk_self_eq_self, validIn_addLatch, Lit.mk_ext]
+  have hlatch := by simp; grind only [addLatch_latches_eq_push, Array.mem_push]
+  have hatom := by simp; grind only [addLatch_matches_atom, validIn_addLatch, Std.HashMap.getElem_insert, addLatch_getElem_eq]
+  ⟨{ aig, map, atomMap, latchNexts, hmap, hlatch, hatom }, by grind only [Array.size_push]⟩
+
+end State
+
+structure Result (stdAig : AIG α) where
   aig : Aig
   refMap : stdAig.Ref -> Lit
   atomMap : α -> Option Var
 
   hrefvalid : ∀ {ref}, refMap ref |>.validIn aig
-  hwf : aig.WF
 
-def fromStdAIG (stdAig : AIG α) (relabel : α -> RelabelledAtom stdAig) : FromStdResult stdAig :=
+end FromStd
+
+open FromStd in
+def fromStdAIG (stdAig : AIG α) (relabel : α -> RelabelledAtom stdAig) : Result stdAig :=
   have ⟨state, hstate⟩ := go
 
-  let aig := state.aig.finaliseLatches fun latch h =>
+  let aig := state.aig.setNexts <| fun latch h =>
     let ref := state.latchNexts[latch.var]'(state.hlatch h)
     have := ref.hgate
-    let lit := state.map[ref.gate]'(by omega) |>.toLit ref.invert
-    ⟨lit, by grind only [Lit.mk_var, Array.getElem_mem]⟩
+    let lit := state.map[ref.gate]'(by omega) |>.invert ref.invert
+    ⟨lit, by grind [!Lit.mk_var]⟩
 
   let refMap (ref : stdAig.Ref) : Lit :=
     have := ref.hgate
-    state.map[ref.gate]'(by omega) |>.toLit ref.invert
+    state.map[ref.gate]'(by omega) |>.invert ref.invert
 
   let atomMap (atom : α) : Option Var := state.atomMap[atom]?
 
   have hrefvalid : ∀ {ref}, refMap ref |>.validIn aig := by
     simp [refMap]
-    grind only [validIn_finaliseLatches, Array.getElem_mem]
+    grind only [validIn_setNexts, Array.getElem_mem]
 
-  { aig, refMap, atomMap, hrefvalid, hwf := finaliseLatches_WF }
+  { aig, refMap, atomMap, hrefvalid }
 
 where
-  go (s : FromStdState stdAig := {}) : { s : FromStdState stdAig // s.map.size ≥ stdAig.decls.size } :=
+  go (s : State stdAig := {}) (h : s.map.size ≤ stdAig.decls.size := by grind) :
+      { s : State stdAig // s.map.size = stdAig.decls.size } :=
     let idx := s.map.size
     if hidx : idx ≥ stdAig.decls.size then 
-      ⟨s, hidx⟩
+      ⟨s, by omega⟩
     else
-      match heq : stdAig.decls[idx] with
-      | .false =>
-        have hmap := by grind only [Array.mem_push, Var.constant_validIn]
-        go { s with map := s.map.push .constant, hmap }
-      | .gate rhs0 rhs1 =>
-        have hdag := stdAig.hdag (i := idx) (lhs := rhs0) (rhs := rhs1) (by omega) heq
-        let rhs0 := s.map[rhs0.gate]'hdag.left |>.toLit rhs0.invert
-        let rhs1 := s.map[rhs1.gate]'hdag.right |>.toLit rhs1.invert
-        let (eq:=_) (aig, lhs) := s.aig.addGate rhs0 rhs1
-        let map := s.map.push lhs.var
+      let ⟨s', h⟩ :=
+        match heq : stdAig.decls[idx] with
+        | .false => s.addFalse
+        | .gate rhs0 rhs1 =>
+          have hdag := @stdAig.hdag idx rhs0 rhs1 (by omega) heq
+          s.addGate rhs0 rhs1 hdag.left hdag.right
+        | .atom atom =>
+          match h : s.tryAddCachedAtom atom with
+          | some s => s
+          | none =>
+            match relabel atom with
+            | .input            symbol => s.addInput atom symbol
+            | .latch next reset symbol => s.addLatch atom next reset symbol
 
-        have hmap := by grind only [addGate_validIn, validIn_addGate, Array.mem_push]
-        have hlatch := by grind only [addGate_latches_eq]
-        have hatom := by grind only [validIn_addGate, addGate_getElem_eq]
-        go { s with aig, map, hmap, hlatch, hatom }
+      have : s'.measure < s.measure := by grind only [State.measure]
+      go s' (by lia)
+  termination_by s.measure
 
-      | .atom atom =>
-        match h : s.atomMap[atom]? with
-        | some var =>
-          let map := s.map.push var
-
-          have hmap := by
-            simp_all
-            rintro _ (hold | hnew)
-            · exact s.hmap hold
-            · have := Std.HashMap.isSome_getElem?_iff_mem.mp (Option.isSome_of_eq_some h)
-              simp_all; rw [←h]; cases (s.hatom this); trivial
-          go { s with map, hmap }
-        | none =>
-          match relabel atom with
-          | .input symbol =>
-            let (eq:=_) (aig, lhs) := s.aig.addInput symbol
-            let map := s.map.push lhs.var
-            let atomMap := s.atomMap.insert atom lhs
-
-            have hmap := by grind only [addInput_validIn, validIn_addInput, Array.mem_push]
-            have hlatch := by grind only [addInput_latches_eq]
-            have hatom := by 
-              intros
-              simp only [Std.HashMap.getElem_insert]
-              split
-              · grind only [addInput_matches_atom]
-              · grind only [validIn_addInput, addInput_getElem_eq]
-            go { s with aig, map, atomMap, hmap, hlatch, hatom }
-
-          | .latch next reset symbol =>
-            let reset := match reset with
-              | .inl bool => Lit.constant bool
-              | .inr var => var.map Lit.ofRef
-
-            let (eq:=_) (aig, lhs) := s.aig.addLatch' reset symbol
-            let map := s.map.push lhs.var
-            let atomMap := s.atomMap.insert atom lhs
-            let latchNexts := s.latchNexts.insert lhs next
-
-            have hmap := by grind only [addLatch'_validIn, validIn_addLatch', Array.mem_push]
-            have hlatch := by grind only [addLatch'_latches_eq_push, Std.HashMap.mem_insert, Array.mem_push]
-            have hatom := by 
-              intros
-              simp only [Std.HashMap.getElem_insert]
-              split
-              · grind only [addLatch'_matches_atom]
-              · grind only [validIn_addLatch', addLatch'_getElem_eq]
-            go { aig, map, atomMap, latchNexts, hmap, hlatch, hatom }
-
-  termination_by stdAig.decls.size - s.map.size
-
+/-
 @[inline]
 def fromStdEntrypoint (entry : Entrypoint α) (relabel : α -> RelabelledAtom entry.aig) :
     (result : FromStdResult entry.aig) × (Lit.In result.aig) :=
   let result := fromStdAIG entry.aig relabel
   let lit := result.refMap entry.ref
   ⟨result, ⟨lit, result.hrefvalid⟩⟩
-
+-/
 
 end Valaig.Aig
