Valaig/ForStd.lean
@@ -1,0 +1,126 @@
+
+namespace Array
+
+variable {α : Type}
+
+-- `Array.modify` doesn't provide a proof that the element being modified corresponds to the index,
+-- but this is often useful so we provide our own implementation, and the unsafe implementation for
+-- performance
+
+@[inline]
+unsafe def modifyMemUnsafe (xs : Array α) (i : Nat) (h : i < xs.size)
+    (f : { a : α // xs[i] = a } → α) : Array α :=
+  let v := xs[i]
+  -- Replace a[i] by `box(0)`.  This ensures that `v` remains unshared if possible.
+  -- Note: we assume that arrays have a uniform representation irrespective
+  -- of the element type, and that it is valid to store `box(0)` in any array.
+  let xs' := xs.set i (unsafeCast ())
+  let v := f ⟨v, by trivial⟩
+  xs'.set i v (by rwa [size_set h])
+
+@[implemented_by modifyMemUnsafe]
+def modifyMem (xs : Array α) (i : Nat) (h : i < xs.size) (f : { a : α // xs[i] = a } → α) : Array α :=
+  xs.set i (f ⟨xs[i], by trivial⟩) h
+
+@[simp, grind =]
+theorem modifyMem_def {xs : Array α} {i : Nat} (h : i < xs.size) (f : { a : α // xs[i] = a } → α) :
+    xs.modifyMem i h f = xs.set i (f ⟨xs[i], by trivial⟩) h := by
+  rw [modifyMem]
+
+@[simp, grind =]
+theorem size_modifyMem {xs : Array α} {i : Nat} (h : i < xs.size) (f : { a : α // xs[i] = a } → α) :
+    (xs.modifyMem i h f).size = xs.size := by
+  rw [modifyMem_def, size_set]
+
+section
+variable {xs xs' : Array α} {i : Nat} {f : (i : Nat) → (h : i < xs.size) → (a : α) → xs[i] = a → α}
+variable {hstep : ∃ h1 h2, xs'[i]'h1 = xs[i]'h2}
+
+@[always_inline]
+private def mapMem.step {xs : Array α} (xs' : Array α) (i : Nat)
+      (f : (i : Nat) → (h : i < xs.size) → (a : α) → xs[i] = a → α)
+      (h : ∃ h1 h2, xs'[i]'h1 = xs[i]'h2) : Array α :=
+    have hxs : i < xs.size := by lia
+    have hxs' : i < xs'.size := by lia
+    xs'.modifyMem i hxs' <| fun ⟨x, p⟩ => f i hxs x (by lia)
+
+private theorem mapMem.step.size_eq : (step xs' i f hstep).size = xs'.size := by
+  grind only [step, size_modifyMem]
+
+private theorem mapMem.step.eq_above {j : Nat} (h1 : j > i) (h2 : j < xs'.size) :
+    (step xs' i f hstep)[j]'(by rw [step.size_eq]; omega) = xs'[j] := by
+  grind only [= getElem_set, step, modifyMem_def]
+
+-- TODO: This can be specialized to use usize for the iterator and also made possible to return
+-- different type
+@[inline]
+def mapMem (xs : Array α) (f : (i : Nat) → (h : i < xs.size) → (a : α) → xs[i] = a → α) : Array α :=
+  @go xs 0 (by omega) (by simp)
+where
+  go (xs' : Array α) (i : Nat) (hsize : xs'.size = xs.size)
+      (heq : ∀ {j} (_ : j ≥ i) (_ : j < xs.size), xs'[j] = xs[j]) :
+      Array α :=
+    if h : i ≥ xs'.size then
+      xs'
+    else
+      let xs' := mapMem.step xs' i f (by grind only)
+
+      have hsize := by rwa [mapMem.step.size_eq]
+      have heq : ∀ {j} (_ : j ≥ i + 1), _ := by grind only [mapMem.step.eq_above]
+      @go xs' (i + 1) hsize heq
+  termination_by xs.size - i
+
+variable {hsize : xs'.size = xs.size}
+variable {hgo : ∀ {j} (_ : j ≥ i) (_ : j < xs.size), xs'[j] = xs[j]}
+
+private theorem mapMem.go.size_eq : (go xs f xs' i hsize hgo).size = xs'.size := by
+  unfold go
+  induction h : (xs.size - i) generalizing xs' i with
+  | zero => lia
+  | succ fuel motive =>
+    split
+    · lia
+    · rw [go, @motive (xs' := step xs' i f (by grind))]
+      · exact step.size_eq
+      · rwa [step.size_eq]
+      · grind only [mapMem.step.eq_above]
+      · omega
+
+private theorem mapMem.go.getElem {j : Nat} (h : j < xs'.size) :
+    (go xs f xs' i hsize hgo)[j]'(by grind only [go.size_eq]) =
+      if _ : j ≥ i then
+        f j (by omega) (xs[j]'(by omega)) rfl
+      else
+        xs'[j] := by
+  unfold go
+  induction h : (xs.size - i) generalizing xs' i with
+  | zero => lia
+  | succ fuel motive =>
+    split
+    · lia
+    · simp
+      unfold go
+      rw [@motive (xs' := step xs' i f (by grind))]
+      · grind only [step, modifyMem_def, getElem_set]
+      · rwa [step.size_eq]
+      · grind only [mapMem.step.eq_above]
+      · rwa [step.size_eq]
+      · omega
+
+@[simp, grind =]
+theorem size_mapMem : (xs.mapMem f).size = xs.size := by
+  apply mapMem.go.size_eq
+  lia
+
+@[simp, grind →]
+theorem getElem_mapMem {i : Nat} (f : (i : Nat) → (h : i < xs.size) → (a : α) → xs[i] = a → α) (hi : i < (xs.mapMem f).size) :
+    have h : i < xs.size := by simp_all
+    (xs.mapMem f)[i] = f i h xs[i] rfl := by
+  unfold mapMem
+  apply mapMem.go.getElem
+  · intros; rfl
+  · rwa [size_mapMem] at hi
+
+end
+
+end Array
