Valaig/Prelude.lean
@@ -1,0 +1,17 @@
+macro:50 "rlet" pat:term ":=" expr:term rest:term : term =>
+  `(match _ : $expr:term with
+      | $pat => $rest)
+
+macro:50 "rlet" h:ident ":" pat:term ":=" expr:term rest:term : term =>
+  `(match $h:ident : $expr:term with
+      | $pat => $rest)
+
+macro:50 "rlet" pat:term "←" expr:term  rest:term : term =>
+  `(match _ : $expr:term with
+      | none => none
+      | some $pat => $rest)
+
+macro:50 "rlet" h:ident ":" pat:term "←" expr:term  rest:term : term =>
+  `(match $h:ident : $expr:term with
+      | none => none
+      | some $pat => $rest)
